Beginning of TypeConstructorsInj.v

theories/DeclarativeSubst.v
@@ -1,7 +1,7 @@
 (** * LogRel.DeclarativeSubst: stability of declarative typing by substitution. *)
 From Coq Require Import CRelationClasses.
 From LogRel.AutoSubst Require Import core unscoped Ast Extra.
-From LogRel Require Import Utils BasicAst Notations Context NormalForms Weakening UntypedReduction
+From LogRel Require Import Utils BasicAst Notations LContexts Context NormalForms Weakening UntypedReduction
   GenericTyping DeclarativeTyping DeclarativeInstance AlgorithmicTyping.
 From LogRel Require Import LogicalRelation Validity Fundamental.
 From LogRel.LogicalRelation Require Import Induction Escape Irrelevance Transitivity.
@@ -14,55 +14,56 @@ Set Printing Primitive Projection Parameters.
 
 Import DeclarativeTypingProperties.
 
-Lemma typing_subst : WfDeclInductionConcl
-  (fun _ => True)
-  (fun Γ A => forall Δ σ, [|- Δ] -> [Δ |-s σ : Γ] -> [Δ |- A[σ]])
-  (fun Γ A t => forall Δ σ, [|- Δ] -> [Δ |-s σ : Γ] -> [Δ |- t[σ] : A[σ]])
-  (fun Γ A B => forall Δ σ σ', [|- Δ] -> [Δ |-s σ ≅ σ' : Γ] -> [Δ |- A[σ] ≅ B[σ']])
-  (fun Γ A t u => forall Δ σ σ', [|- Δ] -> [Δ |-s σ ≅ σ' : Γ] -> [Δ |- t[σ] ≅ u[σ'] : A[σ]]).
+Lemma typing_subst (wl : wfLCon) : WfDeclInductionConcl
+  (fun _ _ => True)
+  (fun wl Γ A => forall Δ σ, [|- Δ]< wl > -> [Δ |-s σ : Γ]< wl > -> [Δ |- A[σ]]< wl >)
+  (fun wl Γ A t => forall Δ σ, [|- Δ]< wl > -> [Δ |-s σ : Γ]< wl > -> [Δ |- t[σ] : A[σ]]< wl >)
+  (fun wl Γ A B => forall Δ σ σ', [|- Δ]< wl > -> [Δ |-s σ ≅ σ' : Γ]< wl > -> [Δ |- A[σ] ≅ B[σ']]< wl >)
+  (fun wl Γ A t u => forall Δ σ σ', [|- Δ]< wl > -> [Δ |-s σ ≅ σ' : Γ]< wl > -> [Δ |- t[σ] ≅ u[σ'] : A[σ]]< wl >) wl.
 Proof.
   unshelve (repeat split ; [shelve|..]).
   - intros Γ ? Ht * HΔ Hσ.
     unshelve eapply Fundamental_subst in Hσ as [].
-    1,3: boundary.
+    3,5: boundary.
+    1: now eapply wfLCon_le_id.
     apply Fundamental in Ht as [VΓ [VA _]].
-    unshelve eapply escape, VA ; tea.
+    unshelve eapply Wescape, VA ; tea.
+    1: now eapply wfLCon_le_id.
     unshelve eapply irrelevanceSubst ; eassumption.
   - intros * Ht * HΔ Hσ.
     unshelve eapply Fundamental_subst in Hσ as [].
-    1,3: boundary.
+    3,5: boundary.
+    1: now eapply wfLCon_le_id.    
     apply Fundamental in Ht as [VΓ [VA] [Vt]].
-    unshelve eapply escapeTerm, Vt ; tea.
+    unshelve eapply WescapeTerm, Vt ; tea.
+    1: now eapply wfLCon_le_id.
     unshelve eapply irrelevanceSubst ; eassumption.
   - intros * Ht * HΔ Hσ.
     unshelve eapply Fundamental_subst_conv in Hσ as [].
-    1,3: boundary.
+    3,5: boundary.
+    1: now eapply wfLCon_le_id.
     apply Fundamental in Ht as [VΓ VA ? Vconv] ; cbn in *.
-    unshelve eapply escapeEq.
-    2: unshelve eapply VA ; tea ; irrValid.
+    unshelve eapply WescapeEq.
+    2: unshelve eapply VA ; tea ; try irrValid.
     cbn.
-    unshelve eapply transEq.
-    6: now apply Vconv.
-    1-2: shelve.
-    + unshelve eapply validTy.
-      4: eapply VB.
-      1: eassumption.
-      irrValid.
-    + unshelve eapply validTy.
-      4: eapply VB.
-      1: eassumption.
-      irrValid.
-    + unshelve irrelevanceRefl.
-      2-3: unshelve eapply VB ; tea.
-      all: irrValid.
+    unshelve eapply WtransEq.
+    5: now apply Vconv.
+    + unshelve (Wirrelevance0 ; [ reflexivity | ]).
+      2-3: unshelve eapply VA ; tea.
+      all: try irrValid.
+      Unshelve.
+      1: now eapply wfLCon_le_id.
+      1: assumption.
+      now irrValid.
   - intros * Ht * HΔ Hσ.
     unshelve eapply Fundamental_subst_conv in Hσ as [].
-    1,3: boundary.
+    3,5: boundary.
+    1: now eapply wfLCon_le_id.
     apply Fundamental in Ht as [VΓ VA Vt Vu Vtu] ; cbn in *.
-    unshelve eapply escapeEqTerm.
-    2: now unshelve eapply VA ; tea ; irrValid.
+    unshelve eapply WescapeEqTerm.
+    2: now unshelve eapply VA ; tea ; try irrValid.
     cbn.
-    eapply transEqTerm.
+    eapply WtransEqTerm.
     + cbn.
       unshelve eapply Vtu.
     + cbn.
@@ -73,19 +74,19 @@ Qed.
 
 Section MoreSubst.
 
-  Lemma ctx_refl Γ :
-    [|- Γ] ->
-    [|- Γ ≅ Γ].
+  Lemma ctx_refl wl Γ :
+    [|- Γ]< wl > ->
+    [|- Γ ≅ Γ]< wl >.
   Proof.
     induction 1.
     all: constructor; tea.
     now econstructor.
   Qed.
 
-  Lemma subst_wk (Γ Δ Δ' : context) (ρ : Δ' ≤ Δ) σ :
-    [|- Δ'] ->
-    [Δ |-s σ : Γ] ->
-    [Δ' |-s σ⟨ρ⟩ : Γ].
+  Lemma subst_wk wl (Γ Δ Δ' : context) (ρ : Δ' ≤ Δ) σ :
+    [|- Δ']< wl > ->
+    [Δ |-s σ : Γ]< wl > ->
+    [Δ' |-s σ⟨ρ⟩ : Γ]< wl >.
   Proof.
     intros ?.
     induction 1 as [|σ Γ A].
@@ -101,10 +102,10 @@ Section MoreSubst.
       reflexivity.
   Qed.
 
-  Corollary well_subst_up (Γ Δ : context) A σ :
-    [Δ |- A] ->
-    [Δ |-s σ : Γ] ->
-    [Δ ,, A |-s σ⟨↑⟩ : Γ].
+  Corollary well_subst_up wl (Γ Δ : context) A σ :
+    [Δ |- A]< wl > ->
+    [Δ |-s σ : Γ]< wl > ->
+    [Δ ,, A |-s σ⟨↑⟩ : Γ]< wl >.
   Proof.
     intros HA Hσ.
     eapply subst_wk with (ρ := wk_step A wk_id) in Hσ.
@@ -115,9 +116,9 @@ Section MoreSubst.
       all: gen_typing.
   Qed.
 
-  Lemma id_subst (Γ : context) :
-    [|- Γ] ->
-    [Γ |-s tRel : Γ].
+  Lemma id_subst wl (Γ : context) :
+    [|- Γ]< wl > ->
+    [Γ |-s tRel : Γ]< wl >.
   Proof.
     induction 1.
     all: econstructor.
@@ -129,63 +130,63 @@ Section MoreSubst.
       cbn ; now renamify.
   Qed.
 
-  Lemma subst_refl (Γ Δ : context) σ :
-    [Γ |-s σ : Δ] ->
-    [Γ |-s σ ≅ σ : Δ].
+  Lemma subst_refl wl (Γ Δ : context) σ :
+    [Γ |-s σ : Δ]< wl > ->
+    [Γ |-s σ ≅ σ : Δ]< wl >.
   Proof.
     induction 1.
     all: econstructor ; tea.
     now eapply TermRefl.
   Qed.
 
-  Theorem typing_subst1 Γ T :
-  (forall (t : term), [Γ |- t : T] ->
-    forall (A : term), [Γ,, T |- A] -> [Γ |- A[t..]]) ×
-  (forall (t : term), [Γ |- t : T] ->
-    forall (A u : term), [Γ,, T |- u : A] -> [Γ |- u[t..] : A[t..]]) ×
-  (forall (t t' : term), [Γ |- t ≅ t' : T] ->
-    forall (A B : term), [Γ,, T |- A ≅ B] -> [Γ |- A[t..] ≅ B[t'..]]) ×
-  (forall (t t' : term), [Γ |- t ≅ t' : T] ->
-    forall (A u v : term), [Γ,, T |- u ≅ v : A] -> [Γ |- u[t..] ≅ v[t'..] : A[t..]]).
+  Theorem typing_subst1 wl Γ T :
+  (forall (t : term), [Γ |- t : T]< wl > ->
+    forall (A : term), [Γ,, T |- A]< wl > -> [Γ |- A[t..]]< wl >) ×
+  (forall (t : term), [Γ |- t : T]< wl > ->
+    forall (A u : term), [Γ,, T |- u : A]< wl > -> [Γ |- u[t..] : A[t..]]< wl >) ×
+  (forall (t t' : term), [Γ |- t ≅ t' : T]< wl > ->
+    forall (A B : term), [Γ,, T |- A ≅ B]< wl > -> [Γ |- A[t..] ≅ B[t'..]]< wl >) ×
+  (forall (t t' : term), [Γ |- t ≅ t' : T]< wl > ->
+    forall (A u v : term), [Γ,, T |- u ≅ v : A]< wl > -> [Γ |- u[t..] ≅ v[t'..] : A[t..]]< wl >).
   Proof.
     repeat match goal with |- _ × _ => split end.
     all: intros * Ht * Hty.
-    all: assert ([|- Γ]) by gen_typing.
-    all: assert ([Γ |-s tRel : Γ]) as Hsubst by now eapply id_subst.
+    all: assert ([|- Γ]< wl >) by gen_typing.
+    all: assert ([Γ |-s tRel : Γ]< wl >) as Hsubst by now eapply id_subst.
     3-4: apply subst_refl in Hsubst.
     all: eapply typing_subst ; tea.
     all: econstructor ; cbn ; refold ; now asimpl.
   Qed.
 
-  Theorem typing_substmap1 Γ T :
-  (forall (t : term), [Γ ,, T |- t : T⟨↑⟩] ->
-    forall (A : term), [Γ,, T |- A] -> 
-      [Γ,, T |- A[t]⇑]) ×
-  (forall (t : term), [Γ ,, T |- t : T⟨↑⟩] ->
-    forall (A u : term), [Γ,, T |- u : A] -> 
-      [Γ,, T |- u[t]⇑ : A[t]⇑]) ×
-  (forall (t t' : term), [Γ ,, T |- t ≅ t' : T⟨↑⟩] ->
-    forall (A B : term), [Γ,, T |- A ≅ B] ->
-      [Γ,, T |- A[t]⇑ ≅ B[t']⇑]) ×
-  (forall (t t' : term), [Γ ,, T |- t ≅ t' : T⟨↑⟩] ->
-    forall (A u v : term), [Γ,, T |- u ≅ v : A] -> 
-      [Γ,, T |- u[t]⇑ ≅ v[t']⇑ : A[t]⇑]).
+  Theorem typing_substmap1 wl Γ T :
+  (forall (t : term), [Γ ,, T |- t : T⟨↑⟩]< wl > ->
+    forall (A : term), [Γ,, T |- A]< wl > -> 
+      [Γ,, T |- A[t]⇑]< wl >) ×
+  (forall (t : term), [Γ ,, T |- t : T⟨↑⟩]< wl > ->
+    forall (A u : term), [Γ,, T |- u : A]< wl > -> 
+      [Γ,, T |- u[t]⇑ : A[t]⇑]< wl >) ×
+  (forall (t t' : term), [Γ ,, T |- t ≅ t' : T⟨↑⟩]< wl > ->
+    forall (A B : term), [Γ,, T |- A ≅ B]< wl > ->
+      [Γ,, T |- A[t]⇑ ≅ B[t']⇑]< wl >) ×
+  (forall (t t' : term), [Γ ,, T |- t ≅ t' : T⟨↑⟩]< wl > ->
+    forall (A u v : term), [Γ,, T |- u ≅ v : A]< wl > -> 
+      [Γ,, T |- u[t]⇑ ≅ v[t']⇑ : A[t]⇑]< wl >).
   Proof.
     repeat match goal with |- _ × _ => split end.
     all: intros * Ht * Hty.
-    all: assert ([|- Γ,, T] × [|- Γ]) as [] by (split; repeat boundary).
-    all : assert (Hsubst : [Γ ,, T |-s ↑ >> tRel : Γ])
+    all: assert ([|- Γ,, T]< wl > × [|- Γ]< wl >) as [] by (split; repeat boundary).
+    all : assert (Hsubst : [Γ ,, T |-s ↑ >> tRel : Γ]< wl >)
             by (change (?x >> ?y) with y⟨x⟩; eapply well_subst_up; [boundary| now eapply id_subst]).
     3-4: apply subst_refl in Hsubst.
     all: eapply typing_subst ; tea.
     all: econstructor ; cbn ; refold; bsimpl; try rewrite <- rinstInst'_term; tea.
   Qed.
 
-  Lemma conv_well_subst1 (Γ : context) A A' :
-    [Γ |- A] ->
-    [Γ |- A'] ->
-    [Γ |- A ≅ A'] ->
-    [Γ,, A |-s tRel : Γ,, A'].
+  Lemma conv_well_subst1 (wl : wfLCon) (Γ : context) A A' :
+    [Γ |- A]< wl > ->
+    [Γ |- A']< wl > ->
+    [Γ |- A ≅ A']< wl > ->
+    [Γ,, A |-s tRel : Γ,, A']< wl >.
   Proof.
     intros HA HA' Hconv.
     econstructor.
@@ -199,21 +200,21 @@ Section MoreSubst.
       gen_typing.
   Qed.
 
-  Theorem stability1 (Γ : context) A A' :
-    [Γ |- A] ->
-    [Γ |- A'] ->
-    [Γ |- A ≅ A'] ->
-    (forall (T : term), [Γ,, A' |-[de] T] -> [Γ,, A |-[de] T])
-    × (forall (T t : term), [Γ,, A' |-[ de ] t : T] -> [Γ,, A |-[de] t : T])
-    × (forall (T T' : term), [Γ,, A' |-[ de ] T ≅ T'] -> [Γ,, A |-[de] T ≅ T'])
+  Theorem stability1 (wl : wfLCon) (Γ : context) A A' :
+    [Γ |- A]< wl > ->
+    [Γ |- A']< wl > ->
+    [Γ |- A ≅ A']< wl > ->
+    (forall (T : term), [Γ,, A' |-[de] T]< wl > -> [Γ,, A |-[de] T]< wl >)
+    × (forall (T t : term), [Γ,, A' |-[ de ] t : T]< wl > -> [Γ,, A |-[de] t : T]< wl >)
+    × (forall (T T' : term), [Γ,, A' |-[ de ] T ≅ T']< wl > -> [Γ,, A |-[de] T ≅ T']< wl >)
     × (forall (T t u : term),
-          [Γ,, A' |-[ de ] t ≅ u : T] -> [Γ,, A |-[de] t ≅ u : T]).
+          [Γ,, A' |-[ de ] t ≅ u : T]< wl > -> [Γ,, A |-[de] t ≅ u : T]< wl >).
   Proof.
     intros * ? ? Hconv.
     eapply (conv_well_subst1 _) in Hconv ; tea.
     pose proof (Hconv' := Hconv).
     apply subst_refl in Hconv'.
-    assert [|- Γ,, A] by gen_typing.
+    assert [|- Γ,, A]< wl > by gen_typing.
     repeat match goal with |- _ × _ => split end.
     all: intros * Hty.
     all: eapply typing_subst in Hty ; tea.
@@ -223,10 +224,10 @@ Section MoreSubst.
 
 End MoreSubst.
 
-Lemma elimSuccHypTy_ty Γ P :
-  [|- Γ] ->
-  [Γ,, tNat |- P] ->
-  [Γ |-[ de ] elimSuccHypTy P].
+Lemma elimSuccHypTy_ty wl Γ P :
+  [|- Γ]< wl > ->
+  [Γ,, tNat |- P]< wl > ->
+  [Γ |-[ de ] elimSuccHypTy P]< wl >.
 Proof.
   intros HΓ HP.
   unfold elimSuccHypTy.
@@ -251,11 +252,11 @@ Proof.
       reflexivity.
 Qed.
 
-Lemma elimSuccHypTy_conv Γ P P' :
-  [|- Γ] ->
-  [Γ,, tNat |- P] ->
-  [Γ,, tNat |- P ≅ P' ] ->
-  [Γ |- elimSuccHypTy P ≅ elimSuccHypTy P'].
+Lemma elimSuccHypTy_conv wl Γ P P' :
+  [|- Γ]< wl > ->
+  [Γ,, tNat |- P]< wl > ->
+  [Γ,, tNat |- P ≅ P' ]< wl > ->
+  [Γ |- elimSuccHypTy P ≅ elimSuccHypTy P']< wl >.
 Proof.
   intros.
   unfold elimSuccHypTy.
@@ -264,20 +265,20 @@ Proof.
   1-2: now constructor.
   eapply convty_simple_arr; tea.
   eapply typing_substmap1; tea.
-  do 2 constructor; refine (wfVar _ (in_here _ _)).
+  do 2 constructor ; unshelve refine (wfVar _ _ (in_here _ _)).
   constructor; boundary.
 Qed.
 
-Lemma conv_well_subst (Γ Δ : context) :
-  [|- Γ] ->
-  [ |- Γ ≅ Δ] ->
-  [Γ |-s tRel : Δ].
+Lemma conv_well_subst wl (Γ Δ : context) :
+  [|- Γ]< wl > ->
+  [ |- Γ ≅ Δ]< wl > ->
+  [Γ |-s tRel : Δ]< wl >.
 Proof.
   intros HΓ.
   induction 1 as [| * ? HA] in HΓ |- *.
   - now econstructor.
-  - assert [Γ |- A] by now inversion HΓ.
-    assert [|- Γ] by now inversion HΓ.
+  - assert [Γ |- A]< wl > by now inversion HΓ.
+    assert [|- Γ]< wl > by now inversion HΓ.
     econstructor ; tea.
     + eapply well_subst_ext, well_subst_up ; eauto.
       reflexivity.
@@ -286,3 +287,40 @@ Proof.
       rewrite <- rinstInst'_term; do 2 erewrite <- wk1_ren_on.
       now eapply typing_wk.
 Qed.
+
+(* Stability and symmetry with redundant hypothesis on the well-formed contexts *)
+
+Section Stability0.
+
+  Let PCon (wl : wfLCon) (Γ : context) := True.
+  Let PTy (wl : wfLCon) (Γ : context) (A : term) := forall Δ,
+    [|-Δ]< wl > -> [|- Δ ≅ Γ]< wl > -> [Δ |- A]< wl >.
+  Let PTm (wl : wfLCon) (Γ : context) (A t : term) := forall Δ,
+    [|-Δ]< wl > -> [|- Δ ≅ Γ]< wl > -> [Δ |- t : A]< wl >.
+  Let PTyEq (wl : wfLCon) (Γ : context) (A B : term) := forall Δ,
+    [|-Δ]< wl > -> [|- Δ ≅ Γ]< wl > -> [Δ |- A ≅ B]< wl >.
+  Let PTmEq (wl : wfLCon) (Γ : context) (A t u : term) := forall Δ,
+    [|-Δ]< wl > -> [|- Δ ≅ Γ]< wl > -> [Δ |- t ≅ u : A]< wl >.
+
+  Theorem stability0 (wl : wfLCon) : WfDeclInductionConcl PCon PTy PTm PTyEq PTmEq wl.
+  Proof.
+    red; prod_splitter; intros Γ * Hty; red.
+    1: easy.
+    all: intros ?? Hconv; eapply (conv_well_subst _) in Hconv ; tea.
+    all: pose proof (Hconv' := Hconv); apply  subst_refl in Hconv'.
+    all: eapply typing_subst in Hty; tea.
+    all: repeat (rewrite idSubst_term in Hty ; [..|reflexivity]).
+    all: eassumption.
+  Qed.
+
+  Definition convCtxSym0 {wl Γ Δ} : [|- Δ]< wl > -> [|-Γ]< wl > -> [|- Δ ≅ Γ]< wl > -> [|- Γ ≅ Δ]< wl >.
+  Proof.
+    induction 3.
+    all: constructor; inversion H; inversion H0; subst; refold.
+    1: now eauto.
+    eapply stability0 ; tea.
+    1: now symmetry.
+    now eauto.
+  Qed.
+
+End Stability0.
