theories/TypeConstructorsInj.v
@@ -1,67 +1,56 @@
 (** * LogRel.TypeConstructorsInj: injectivity and no-confusion of type constructors, and many consequences, including subject reduction. *)
 From Coq Require Import CRelationClasses.
 From LogRel.AutoSubst Require Import core unscoped Ast Extra.
-From LogRel Require Import Utils BasicAst Notations Context NormalForms Weakening UntypedReduction
-  GenericTyping DeclarativeTyping DeclarativeInstance AlgorithmicTyping.
-From LogRel Require Import LogicalRelation Validity Fundamental DeclarativeSubst.
-From LogRel.LogicalRelation Require Import Escape Neutral Induction.
-From LogRel.Substitution Require Import Escape.
-
+From LogRel Require Import Utils BasicAst Notations LContexts Context NormalForms Weakening UntypedReduction
+  GenericTyping DeclarativeTyping DeclarativeInstance.
+From LogRel Require Import Monad LogicalRelation Validity Fundamental DeclarativeSubst.
+From LogRel.LogicalRelation Require Import Escape Irrelevance Neutral Induction NormalRed Split.
+From LogRel.Substitution Require Import Escape Monotonicity Poly.
+From LogRel.Substitution.Introductions Require Import Pi Sigma.
+                                       
 Set Printing Primitive Projection Parameters.
 
 Import DeclarativeTypingProperties.
 
-
 Section TypeConstructors.
 
-  Definition type_hd_view (Γ : context) {T T' : term} (nfT : isType T) (nfT' : isType T') : Type :=
+  Definition type_hd_view (wl : wfLCon) (Γ : context) {T T' : term} (nfT : isType T) (nfT' : isType T') : Type :=
     match nfT, nfT' with
       | @UnivType s, @UnivType s' => s = s'
-      | @ProdType A B, @ProdType A' B' => [Γ |- A' ≅ A] × [Γ,, A' |- B ≅ B']
+      | @ProdType A B, @ProdType A' B' => [Γ |- A' ≅ A]< wl > × [Γ,, A' |- B ≅ B']< wl >
+      | BoolType, BoolType => True
       | NatType, NatType => True
       | EmptyType, EmptyType => True
-      | NeType _, NeType _ => [Γ |- T ≅ T' : U]
+      | NeType _, NeType _ => [Γ |- T ≅ T' : U]< wl >
+      | @SigType A B, @SigType A' B' => [Γ |- A' ≅ A]< wl > × [Γ,, A' |- B ≅ B']< wl >
+      | @IdType A x y, @IdType A' x' y' => [× [Γ |- A' ≅ A]< wl >, [Γ |- x ≅ x' : A]< wl > & [Γ |- y ≅ y' : A]< wl >]
       | _, _ => False
     end.
 
-  Lemma red_ty_complete : forall (Γ : context) (T T' : term),
-    isType T ->
-    [Γ |- T ≅ T'] ->
-    ∑ T'', [Γ |- T' ⇒* T''] × isType T''.
+  Lemma type_hd_view_over_tree (wl : wfLCon) (Γ : context) {T T' : term} (nfT : isType T) (nfT' : isType T') (d : DTree wl) :
+    (forall wl', over_tree wl wl' d -> type_hd_view wl' Γ nfT nfT') ->
+    type_hd_view wl Γ nfT nfT'.
   Proof.
-    intros * tyT Hconv.
-    eapply Fundamental in Hconv as [HΓ HT HT' Hconv].
-    eapply reducibleTyEq in Hconv.
-    set (HTred := reducibleTy _ HT) in *.
-    clearbody HTred.
-    clear HT.
-    destruct HTred as [[] lr] ; cbn in *.
-    destruct lr.
-    - destruct Hconv as [[]].
-      eexists ; split; tea.
-      constructor.
-    - destruct Hconv as [? red].
-      eexists ; split.
-      1: apply red.
-      apply ty_ne_whne in ne.
-      now constructor.
-    - destruct Hconv as [?? red].
-      eexists ; split.
-      1: apply red.
-      now constructor.
-    - destruct Hconv as [red].
-      eexists ; split.
-      1: apply red.
-      now constructor.
-    - destruct Hconv as [red].
-      eexists ; split.
-      1: apply red.
-      now constructor.
-  Qed.
+    eapply split_to_over_tree.
+    clear wl d ; intros wl n ne.
+    destruct nfT, nfT' ; cbn ; eauto.
+    - intros [HAt HBt] [HAf HBf] ; split.
+      + now eapply ϝTypeConv. 
+      + now eapply ϝTypeConv. 
+    - intros [HAt HBt] [HAf HBf] ; split.
+      + now eapply ϝTypeConv. 
+      + now eapply ϝTypeConv.
+    - intros [HAt HBt] [HAf HBf] ; split.
+      + now eapply ϝTypeConv. 
+      + now eapply ϝTermConv. 
+      + now eapply ϝTermConv.
+    - intros HAt HAf.
+      now eapply ϝTermConv. 
+  Qed.                
 
-  Lemma ty_conv_inj : forall (Γ : context) (T T' : term) (nfT : isType T) (nfT' : isType T'),
-    [Γ |- T ≅ T'] ->
-    type_hd_view Γ nfT nfT'.
+  Lemma ty_conv_inj : forall (wl : wfLCon) (Γ : context) (T T' : term) (nfT : isType T) (nfT' : isType T'),
+    [Γ |- T ≅ T']< wl > ->
+    type_hd_view wl Γ nfT nfT'.
   Proof.
     intros * Hconv.
     eapply Fundamental in Hconv as [HΓ HT HT' Hconv].
@@ -70,110 +59,154 @@ Section TypeConstructors.
     clearbody HTred.
     clear HT.
     eapply reducibleTy in HT'.
-    destruct HTred as [[] lrT].
-    cbn in *.
-    inversion lrT ; subst ; clear lrT.
-    - subst.
-      destruct Hconv as [].
+    unshelve eapply type_hd_view_over_tree.
+    1: eapply DTree_fusion ; [eapply DTree_fusion | ] ; shelve.
+    intros wl' Ho.
+    pose proof (HTRed := WRed _ HTred _ (over_tree_fusion_l (over_tree_fusion_l Ho))).
+    assert (HConv : [HTRed | Γ ||- T ≅ T' ]< wl' >).
+    { irrelevanceRefl ; unshelve eapply Hconv.
+      1: now eapply (over_tree_fusion_l (over_tree_fusion_l Ho)).
+      now eapply (over_tree_fusion_r Ho).
+    }
+    assert (HΓ' : [||-v Γ ]< wl' >).
+    { eapply WfC_Ltrans ; eauto.
+      now eapply over_tree_le.
+    }
+    clear HΓ.
+    pose proof (HTRed' := WRed _ HT' _ (over_tree_fusion_r (over_tree_fusion_l Ho))).
+    clear HTred HT' Hconv Ho.
+    revert nfT T' nfT' HΓ' HTRed' HConv. 
+    revert HTRed. 
+    generalize (eq_refl : one = one).
+    generalize one at 1 3 ; intros l eql HTred; revert eql.
+    pattern l, wl', Γ, T, HTred ; apply LR_rect_TyUr ; clear l wl wl' Γ T HTred.
+    all: intros ? wl Γ T.
+    - intros [] -> nfT T' nfT' HΓ HT' [].
       assert (T' = U) as HeqT' by (eapply redtywf_whnf ; gen_typing); subst.
-      destruct H.
       assert (T = U) as HeqU by (eapply redtywf_whnf ; gen_typing). 
       destruct nfT ; inversion HeqU ; subst.
       2: now exfalso ; gen_typing.
       clear HeqU.
+      Set Printing All.
       remember U as T eqn:HeqU in nfT' |- * at 2.
-      destruct nfT' ; inversion HeqU ; subst.
+      destruct nfT'; inversion HeqU ; subst.
       2: now exfalso ; gen_typing.
       now reflexivity.
-    - destruct neA as [nT ? ne], Hconv as [nT' ? ne'] ; cbn in *.
+    - Unset Printing All.
+      intros [nT ? ne] -> nfT T' nfT' HΓ HT' [nT' ? ne']; cbn in *.
       assert (T = nT) as <- by
-        (apply red_whnf ; gen_typing).
+        (apply (red_whnf (l := wl)) ; gen_typing).
       assert (T' = nT') as <- by
-        (apply red_whnf ; gen_typing).
+        (apply (red_whnf (l:= wl)) ; gen_typing).
       destruct nfT.
-      + apply ty_ne_whne in ne, ne'; exfalso ; gen_typing.
-      + apply ty_ne_whne in ne, ne'; exfalso ; gen_typing.
-      + apply ty_ne_whne in ne, ne'; inversion ne.
-      + destruct nfT'.
-        * apply ty_ne_whne in ne, ne'; exfalso ; gen_typing.
-        * apply ty_ne_whne in ne, ne'; exfalso ; gen_typing.
-        * apply ty_ne_whne in ne, ne'; inversion ne'.
-        * apply ty_ne_whne in ne, ne'; inversion ne'; gen_typing.
-        * apply ty_ne_whne in ne, ne'. inversion ne.
-      + destruct nfT'.
-        * apply ty_ne_whne in ne, ne'; exfalso ; gen_typing.
-        * apply ty_ne_whne in ne, ne'; exfalso ; gen_typing.
-        * apply ty_ne_whne in ne, ne'; inversion ne'.
-        * apply ty_ne_whne in ne, ne'; inversion ne'; gen_typing.
-        * apply ty_ne_whne in ne, ne'. cbn. gen_typing.
-    - assert [|- Γ] by (apply escape in HT' ; boundary).
-      rewrite <- (PiRedTyPack.pack_beta ΠA ΠAad) in *.
-      remember (PiRedTyPack.pack ΠA ΠAad) as ΠA' eqn:Heq in *.
-      clear ΠA ΠAad Heq.
-      destruct ΠA' as [dom cod red], Hconv as [dom' cod' red'] ; cbn in *.
-      assert (T = tProd dom cod) as HeqT by (apply red_whnf ; gen_typing). 
-      assert (T' = tProd dom' cod') as HeqT' by (apply red_whnf ; gen_typing).
-      destruct nfT.
-      1,3,4: congruence.
-      2: subst ; exfalso ; gen_typing.
+      1-7: apply convneu_whne in ne; inversion ne.
       destruct nfT'.
-      1,3,4: congruence.
-      2: subst ; exfalso ; gen_typing.
-      inversion HeqT ; inversion HeqT' ; subst ; clear HeqT HeqT'.
-      cbn.
-      assert [Γ |-[ de ] dom' ≅ dom].
-      {
-        symmetry.
-        replace dom with (dom⟨wk_id (Γ := Γ)⟩) by now bsimpl.
-        replace dom' with (dom'⟨wk_id (Γ := Γ)⟩) by now bsimpl.
-        now unshelve now eapply LogicalRelation.Escape.escapeEq.
-      }
-      split ; tea.
-      replace cod with (cod[tRel 0 .: (wk1 (Γ := Γ) dom') >> tRel ])
-        by (bsimpl ; rewrite scons_eta' ; now bsimpl).
-      replace cod' with (cod'[tRel 0 .: (wk1 (Γ := Γ) dom') >> tRel ])
-        by (bsimpl ; rewrite scons_eta' ; now bsimpl).
-      assert [ |-[ de ] Γ,, dom'].
-      {
-        econstructor ; tea.
-        eapply prod_ty_inv.
-        now gen_typing.
-      }
-      (unshelve now eapply LogicalRelation.Escape.escapeEq) ; tea.
-      apply neuTerm.
-      1: econstructor; reflexivity.
-      2: econstructor.
-      1,2: eapply wfTermConv.
-      2,4: eapply typing_wk; tea.
-      1,2: rewrite wk1_ren_on; constructor; tea; constructor.
-    - destruct Hconv.
-      assert (T' = tNat) as HeqT' by (eapply redtywf_whnf ; gen_typing).
-      assert (T = tNat) as HeqT by (destruct NA; eapply redtywf_whnf ; gen_typing).
+      1-7: symmetry in ne'; apply convneu_whne in ne'; inversion ne'.
+      cbn. all: cbn ; try now gen_typing.
+    - intros [dom cod red] _ _ -> nfT T' nfT' HΓ HT'[dom' cod' red']; cbn in *.
+      assert (T = tProd dom cod) as HeqT by (apply (red_whnf (l := wl)) ; gen_typing). 
+      assert (T' = tProd dom' cod') as HeqT' by (apply (red_whnf (l := wl)) ; gen_typing).
+      destruct nfT; cycle -1.
+      1: subst ; exfalso ; gen_typing.
+      all: try congruence.
+      destruct nfT'; cycle -1.
+      1: subst ; exfalso ; gen_typing.
+      all: try congruence.
+      inversion HeqT ; inversion HeqT' ; subst ; clear HeqT HeqT'; cbn.
+      destruct (polyRedEqId (normRedΠ0 (invLRΠ HT')) (PolyRedEqSym _ polyRed0)).
+      split; now Wescape.
+    - intros [] -> nfT T' nfT' HΓ HT' [].
+      assert (T' = tNat) as HeqT' by (eapply (redtywf_whnf (l:= wl)) ; gen_typing).
+      assert (T = tNat) as HeqT by (eapply (redtywf_whnf (l:= wl)) ; gen_typing).
       destruct nfT; inversion HeqT.
       + destruct nfT'; inversion HeqT'.
         * constructor.
         * exfalso; subst; inversion w.
       + exfalso; subst; inversion w.
-    - destruct Hconv.
-      assert (T' = tEmpty) as HeqT' by (eapply redtywf_whnf ; gen_typing).
-      assert (T = tEmpty) as HeqT by (destruct NA; eapply redtywf_whnf ; gen_typing).
+    - intros [] -> nfT T' nfT' HΓ HT' [].
+      assert (T' = tBool) as HeqT' by (eapply (redtywf_whnf (l:= wl)) ; gen_typing).
+      assert (T = tBool) as HeqT by (eapply (redtywf_whnf (l:= wl)) ; gen_typing).
+      destruct nfT; inversion HeqT.
+      + destruct nfT'; inversion HeqT'.
+        * constructor.
+        * exfalso; subst; inversion w.
+      + exfalso; subst; inversion w.
+    - intros [] -> nfT T' nfT' HΓ HT' [].
+      assert (T' = tEmpty) as HeqT' by (eapply (redtywf_whnf (l:= wl)) ; gen_typing).
+      assert (T = tEmpty) as HeqT by (eapply (redtywf_whnf (l:= wl)) ; gen_typing).
       destruct nfT; inversion HeqT.
       + destruct nfT'; inversion HeqT'.
         * econstructor.
         * exfalso; subst; inversion w.
       + exfalso; subst; inversion w.
+    - intros [dom cod red] _ _ -> nfT T' nfT' HΓ HT' [dom' cod' red'].
+      assert (T = tSig dom cod) as HeqT by (apply (red_whnf (l:= wl)) ; gen_typing). 
+      assert (T' = tSig dom' cod') as HeqT' by (apply (red_whnf (l:= wl)) ; gen_typing).
+      destruct nfT; cycle -1.
+      1: subst; inv_whne.
+      all: try congruence.
+      destruct nfT'; cycle -1.
+      1: subst; inv_whne.
+      all: try congruence.
+      inversion HeqT ; inversion HeqT' ; subst ; clear HeqT HeqT'; cbn.
+      destruct (polyRedEqId (normRedΣ0 (invLRΣ HT')) (PolyRedEqSym _ polyRed0)).
+      split; now Wescape.
+    - intros [??? ty] _ _ -> nfT T' nfT' HΓ HT' [??? ty']; cbn in *.
+      assert (T = ty) as HeqT by (apply (red_whnf (l:= wl)); gen_typing).
+      assert (T' = ty') as HeqT' by (apply (red_whnf (l:= wl)); gen_typing).
+      destruct nfT; cycle -1; [subst; inv_whne|..]; unfold ty in *; try congruence.
+      destruct nfT'; cycle -1; [subst; inv_whne|..]; unfold ty' in *; try congruence.
+      cbn; inversion HeqT; inversion HeqT'; subst; escape; now split.
   Qed.
 
+(*
+    
+  Lemma red_ty_complete : forall (wl : wfLCon) (Γ : context) (T T' : term),
+    isType T ->
+    [Γ |- T ≅ T']< wl > ->
+    ∑ d T'', isType T'' × (forall wl', over_tree wl wl' d -> [Γ |- T' ⤳* T'']< wl' >).
+ Proof.
+   intros * tyT Hconv.
+   eapply Fundamental in Hconv as [HΓ HT HT' Hconv].
+   eapply reducibleTyEq in Hconv.
+   set (HTred := reducibleTy _ HT) in *.
+   clearbody HTred.
+   clear HT.
+   assert (Hyp : forall d : DTree wl,
+              Ssig (fun wl' : wfLCon => over_tree wl wl' d)).
+   { clear.
+     induction d.
+     - exists k.
+       now eapply wfLCon_le_id.
+     - cbn.
+       clear IHd2 ; destruct IHd1 as [wl' Hyp].
+       exists wl'.
+       pose (H := over_tree_le Hyp _ _ (in_here_l _)).
+       now rewrite (decidInLCon_true H).
+   }
+   pose (d := DTree_fusion _ (WT _ HTred) (WTEq _ Hconv)).
+   specialize (Hyp d) ; destruct Hyp as [wl' Hwl'].
+
+   
+    exists (DTree_fusion _ (WT _ HTred) (WTEq _ Hconv)).
+    destruct HTred as [d HTred].
+    destruct HTred as [[] lr] ; cbn in *.
+    destruct lr.
+    all: destruct Hconv; eexists; split; [lazymatch goal with H : [_ |- _ :⤳*: _] |- _ => apply H end|]; constructor.
+    eapply convneu_whne; now symmetry.
+  Qed.
+
+
   Corollary red_ty_compl_univ_l Γ T :
-    [Γ |- U ≅ T] ->
-    [Γ |- T ⇒* U].
+    [Γ |- U ≅ T]< wl > ->
+    [Γ |- T ⤳* U]< wl >.
   Proof.
     intros HT.
     pose proof HT as HT'.
     unshelve eapply red_ty_complete in HT' as (T''&[? nfT]).
     2: econstructor.
     enough (T'' = U) as -> by easy.
-    assert [Γ |- U ≅ T''] as Hconv by
+    assert [Γ |- U ≅ T'']< wl > as Hconv by
       (etransitivity ; [eassumption|now eapply RedConvTyC]).
     unshelve eapply ty_conv_inj in Hconv.
     1: econstructor.
@@ -182,8 +215,8 @@ Section TypeConstructors.
   Qed.
 
   Corollary red_ty_compl_univ_r Γ T :
-    [Γ |- T ≅ U] ->
-    [Γ |- T ⇒* U].
+    [Γ |- T ≅ U]< wl > ->
+    [Γ |- T ⤳* U]< wl >.
   Proof.
     intros.
     eapply red_ty_compl_univ_l.
@@ -191,15 +224,15 @@ Section TypeConstructors.
   Qed.
 
   Corollary red_ty_compl_nat_l Γ T :
-    [Γ |- tNat ≅ T] ->
-    [Γ |- T ⇒* tNat].
+    [Γ |- tNat ≅ T]< wl > ->
+    [Γ |- T ⤳* tNat]< wl >.
   Proof.
     intros HT.
     pose proof HT as HT'.
     unshelve eapply red_ty_complete in HT' as (T''&[? nfT]).
     2: econstructor.
     enough (T'' = tNat) as -> by easy.
-    assert [Γ |- tNat ≅ T''] as Hconv by
+    assert [Γ |- tNat ≅ T'']< wl > as Hconv by
       (etransitivity ; [eassumption|now eapply RedConvTyC]).
     unshelve eapply ty_conv_inj in Hconv.
     1: econstructor.
@@ -208,8 +241,8 @@ Section TypeConstructors.
   Qed.
 
   Corollary red_ty_compl_nat_r Γ T :
-    [Γ |- T ≅ tNat] ->
-    [Γ |- T ⇒* tNat].
+    [Γ |- T ≅ tNat]< wl > ->
+    [Γ |- T ⤳* tNat]< wl >.
   Proof.
     intros.
     eapply red_ty_compl_nat_l.
@@ -217,15 +250,15 @@ Section TypeConstructors.
   Qed.
 
   Corollary red_ty_compl_empty_l Γ T :
-    [Γ |- tEmpty ≅ T] ->
-    [Γ |- T ⇒* tEmpty].
+    [Γ |- tEmpty ≅ T]< wl > ->
+    [Γ |- T ⤳* tEmpty]< wl >.
   Proof.
     intros HT.
     pose proof HT as HT'.
     unshelve eapply red_ty_complete in HT' as (T''&[? nfT]).
     2: econstructor.
     enough (T'' = tEmpty) as -> by easy.
-    assert [Γ |- tEmpty ≅ T''] as Hconv by
+    assert [Γ |- tEmpty ≅ T'']< wl > as Hconv by
       (etransitivity ; [eassumption|now eapply RedConvTyC]).
     unshelve eapply ty_conv_inj in Hconv.
     1: econstructor.
@@ -234,8 +267,8 @@ Section TypeConstructors.
   Qed.
 
   Corollary red_ty_compl_empty_r Γ T :
-    [Γ |- T ≅ tEmpty] ->
-    [Γ |- T ⇒* tEmpty].
+    [Γ |- T ≅ tEmpty]< wl > ->
+    [Γ |- T ⤳* tEmpty]< wl >.
   Proof.
     intros.
     eapply red_ty_compl_empty_l.
@@ -243,14 +276,14 @@ Section TypeConstructors.
   Qed.
 
   Corollary red_ty_compl_prod_l Γ A B T :
-    [Γ |- tProd A B ≅ T] ->
-    ∑ A' B', [× [Γ |- T ⇒* tProd A' B'], [Γ |- A' ≅ A] & [Γ,, A' |- B ≅ B']].
+    [Γ |- tProd A B ≅ T]< wl > ->
+    ∑ A' B', [× [Γ |- T ⤳* tProd A' B']< wl >, [Γ |- A' ≅ A]< wl > & [Γ,, A' |- B ≅ B']< wl >].
   Proof.
     intros HT.
     pose proof HT as HT'.
     unshelve eapply red_ty_complete in HT as (T''&[? nfT]).
     2: econstructor.
-    assert [Γ |- tProd A B ≅ T''] as Hconv by 
+    assert [Γ |- tProd A B ≅ T'']< wl > as Hconv by 
       (etransitivity ; [eassumption|now eapply RedConvTyC]).
     unshelve eapply ty_conv_inj in Hconv.
     1: constructor.
@@ -261,8 +294,8 @@ Section TypeConstructors.
   Qed.
 
   Corollary prod_ty_inj Γ A B  A' B' :
-    [Γ |- tProd A B ≅ tProd A' B'] ->
-    [Γ |- A' ≅ A] × [Γ,, A' |- B ≅ B'].
+    [Γ |- tProd A B ≅ tProd A' B']< wl > ->
+    [Γ |- A' ≅ A]< wl > × [Γ,, A' |- B ≅ B']< wl >.
   Proof.
     intros Hty.
     unshelve eapply ty_conv_inj in Hty.
@@ -270,14 +303,83 @@ Section TypeConstructors.
     now eassumption.
   Qed.
 
+  Corollary red_ty_compl_sig_l Γ A B T :
+    [Γ |- tSig A B ≅ T]< wl > ->
+    ∑ A' B', [× [Γ |- T ⤳* tSig A' B']< wl >, [Γ |- A' ≅ A]< wl > & [Γ,, A' |- B ≅ B']< wl >].
+  Proof.
+    intros HT.
+    pose proof HT as HT'.
+    unshelve eapply red_ty_complete in HT as (T''&[? nfT]).
+    2: econstructor.
+    assert [Γ |- tSig A B ≅ T'']< wl > as Hconv by 
+      (etransitivity ; [eassumption|now eapply RedConvTyC]).
+    unshelve eapply ty_conv_inj in Hconv.
+    1: constructor.
+    1: assumption.
+    destruct nfT, Hconv.
+    do 2 eexists ; split.
+    all: eassumption.
+  Qed.
+  
+  Corollary red_ty_compl_sig_r Γ A B T :
+    [Γ |- T ≅ tSig A B]< wl > ->
+    ∑ A' B', [× [Γ |- T ⤳* tSig A' B']< wl >, [Γ |- A' ≅ A]< wl > & [Γ,, A' |- B ≅ B']< wl >].
+  Proof.
+    intros; eapply red_ty_compl_sig_l; now symmetry.
+  Qed.
+
+  Corollary sig_ty_inj Γ A B  A' B' :
+    [Γ |- tSig A B ≅ tSig A' B']< wl > ->
+    [Γ |- A' ≅ A]< wl > × [Γ,, A' |- B ≅ B']< wl >.
+  Proof.
+    intros Hty.
+    unshelve eapply ty_conv_inj in Hty.
+    1-2: constructor.
+    now eassumption.
+  Qed.
+
+  Corollary red_ty_compl_id_l Γ A x y T :
+    [Γ |- tId A x y ≅ T]< wl > ->
+    ∑ A' x' y', [× [Γ |- T ⤳* tId A' x' y']< wl >, [Γ |- A' ≅ A]< wl >, [Γ |- x ≅ x' : A]< wl > & [Γ |- y ≅ y' : A]< wl >].
+  Proof.
+    intros HT.
+    pose proof HT as HT'.
+    unshelve eapply red_ty_complete in HT as (T''&[? nfT]).
+    2: econstructor.
+    assert [Γ |- tId A x y ≅ T'']< wl > as Hconv by 
+      (etransitivity ; [eassumption|now eapply RedConvTyC]).
+    unshelve eapply ty_conv_inj in Hconv.
+    1: constructor.
+    1: assumption.
+    destruct nfT, Hconv.
+    do 3 eexists ; split; eassumption.
+  Qed.
+  
+  Corollary red_ty_compl_id_r Γ A x y T :
+    [Γ |- T ≅ tId A x y]< wl > ->
+    ∑ A' x' y', [× [Γ |- T ⤳* tId A' x' y']< wl >, [Γ |- A' ≅ A]< wl >, [Γ |- x ≅ x' : A]< wl > & [Γ |- y ≅ y' : A]< wl >].
+  Proof.
+    intros; eapply red_ty_compl_id_l; now symmetry.
+  Qed.
+
+  Corollary id_ty_inj {Γ A A' x x' y y'} :
+    [Γ |- tId A x y ≅ tId A' x' y']< wl > ->
+    [× [Γ |- A' ≅ A]< wl >, [Γ |- x ≅ x' : A]< wl > & [Γ |- y ≅ y' : A]< wl >].
+  Proof.
+    intros Hty.
+    unshelve eapply ty_conv_inj in Hty.
+    1-2: constructor.
+    now eassumption.
+  Qed.
+*)
 End TypeConstructors.
 
 Section Boundary.
 
-  Lemma in_ctx_wf Γ n decl :
-    [|- Γ] ->
+  Lemma in_ctx_wf wl Γ n decl :
+    [|- Γ]< wl > ->
     in_ctx Γ n decl ->
-    [Γ |- decl].
+    [Γ |- decl]< wl >.
   Proof.
     intros HΓ Hin.
     induction Hin.
@@ -289,147 +391,131 @@ Section Boundary.
       now eapply typing_wk.
   Qed.
 
-  Let PCon (Γ : context) := True.
-  Let PTy (Γ : context) (A : term) := True.
-  Let PTm (Γ : context) (A t : term) := [Γ |- A].
-  Let PTyEq (Γ : context) (A B : term) := [Γ |- A] × [Γ |- B].
-  Let PTmEq (Γ : context) (A t u : term) := [× [Γ |- A], [Γ |- t : A] & [Γ |- u : A]].
+  Lemma scons2_well_subst {wl Γ A B} : 
+    (forall a b, [Γ |- a : A]< wl > -> [Γ |- b : B[a..]]< wl > -> [Γ |-s (b .: a ..) : (Γ ,, A),, B]< wl >)
+    × (forall a a' b b', [Γ |- a ≅ a' : A]< wl > -> [Γ |- b ≅ b' : B[a..]]< wl > -> [Γ |-s (b .: a..) ≅ (b' .: a'..) : (Γ ,, A),, B]< wl >).
+  Proof.
+    assert (h : forall (a : term) σ, ↑ >> (a .: σ) =1 σ) by reflexivity.
+    assert (h' : forall a σ t, t[↑ >> (a .: σ)] = t[σ]) by (intros; now setoid_rewrite h).
+    split; intros; econstructor.
+    - asimpl; econstructor.
+      2: cbn; rewrite h'; now asimpl.
+      asimpl; eapply id_subst; gen_typing.
+    - cbn; now rewrite h'.
+    - asimpl; econstructor.
+      2: cbn; rewrite h'; now asimpl.
+      asimpl; eapply subst_refl; eapply id_subst; gen_typing.
+    - cbn; now rewrite h'.
+  Qed.
 
-  Lemma boundary : WfDeclInductionConcl PCon PTy PTm PTyEq PTmEq.
+  Lemma typing_subst2 {wl Γ A B} :
+    [|- Γ]< wl > ->
+    (forall P a b, [Γ |- a : A]< wl > -> [Γ |- b : B[a..]]< wl > -> [Γ,, A,, B |- P]< wl > -> [Γ |- P[b .: a ..]]< wl >)
+    × (forall P P' a a' b b', [Γ |- a ≅ a' : A]< wl > -> [Γ |- b ≅ b' : B[a..]]< wl > -> [Γ,, A ,, B |- P ≅ P']< wl > -> [Γ |- P[b .: a..] ≅ P'[b' .: a'..]]< wl >).
+  Proof.
+    intros;split; intros; eapply typing_subst; tea; now eapply scons2_well_subst.
+  Qed.
+
+  Lemma shift_subst_eq t a : t⟨↑⟩[a..] = t.
+  Proof. now asimpl. Qed.
+
+  Lemma idElimMotiveCtx {wl Γ A x} : 
+    [Γ |- A]< wl > ->
+    [Γ |- x : A]< wl > ->
+    [|- (Γ,, A),, tId A⟨@wk1 Γ A⟩ x⟨@wk1 Γ A⟩ (tRel 0)]< wl >.
+  Proof.
+    intros; assert [|- Γ]< wl > by boundary.
+    assert [|- Γ,, A]< wl > by now econstructor.
+    econstructor; tea.
+    econstructor.
+    1: now eapply wft_wk. 
+    1:  eapply ty_wk; tea; econstructor; tea.
+    rewrite wk1_ren_on; now eapply ty_var0.
+  Qed.
+
+  Lemma idElimMotiveCtxConv {wl Γ Γ' A A' x x'} :
+    [|- Γ ≅ Γ']< wl > ->
+    [Γ |- A ≅ A']< wl > ->
+    [Γ |- x ≅ x' : A]< wl > ->
+    [ |- (Γ,, A),, tId A⟨@wk1 Γ A⟩ x⟨@wk1 Γ A⟩ (tRel 0)]< wl > ->
+    [ |- (Γ',, A'),, tId A'⟨@wk1 Γ' A'⟩ x'⟨@wk1 Γ' A'⟩ (tRel 0)]< wl > ->
+    [ |- (Γ',, A'),, tId A'⟨@wk1 Γ' A'⟩ x'⟨@wk1 Γ' A'⟩ (tRel 0) ≅ (Γ,, A),, tId A⟨@wk1 Γ A⟩ x⟨@wk1 Γ A⟩ (tRel 0)]< wl >.
+  Proof.
+    intros.
+    assert [|- Γ]< wl > by boundary.
+    assert [Γ |- A]< wl > by boundary.
+    eapply convCtxSym0; tea.
+    econstructor.
+    1: econstructor; tea; now eapply ctx_refl.
+    erewrite (wk1_irr (t:=A')), (wk1_irr (t:=x')); econstructor.
+    1,2: eapply typing_wk; tea; gen_typing.
+    rewrite wk1_ren_on; eapply TermRefl; now eapply ty_var0.
+  Qed.
+
+  Let PCon (wl : wfLCon) (Γ : context) := True.
+  Let PTy (wl : wfLCon) (Γ : context) (A : term) := True.
+  Let PTm (wl : wfLCon) (Γ : context) (A t : term) := [Γ |- A]< wl >.
+  Let PTyEq (wl : wfLCon) (Γ : context) (A B : term) := [Γ |- A]< wl > × [Γ |- B]< wl >.
+  Let PTmEq (wl : wfLCon) (Γ : context) (A t u : term) := [× [Γ |- A]< wl >, [Γ |- t : A]< wl > & [Γ |- u : A]< wl >].
+
+  Lemma boundary (wl : wfLCon) : WfDeclInductionConcl PCon PTy PTm PTyEq PTmEq wl.
   Proof.
     subst PCon PTy PTm PTyEq PTmEq.
-    apply WfDeclInduction.
-    all: try easy.
-    - intros.
-      now eapply in_ctx_wf.
-    - intros.
-      now econstructor.
-    - intros.
-      now eapply typing_subst1, prod_ty_inv.
-    - intros; gen_typing.
-    - intros; gen_typing.
-    - intros.
-      now eapply typing_subst1.
-    - intros; gen_typing.
-    - intros.
-      now eapply typing_subst1.
-    - intros * ? _ ? [] ? [].
-      split.
-      all: constructor ; tea.
-      eapply stability1.
-      3: now symmetry.
-      all: eassumption.
-    - intros * ? [].
-      split.
-      all: now econstructor.
-    - intros.
-      split.
-      + now eapply typing_subst1.
-      + econstructor ; tea.
-        now econstructor.
-      + now eapply typing_subst1.
-    - intros * ? _ ? [] ? [].
-      split.
-      + easy.
-      + now econstructor.
-      + econstructor ; tea.
-        eapply stability1.
-        4: eassumption.
-        all: econstructor ; tea.
-        now symmetry.
-    - intros * ? [] ? [].
-      split.
-      + eapply typing_subst1.
-        1: eassumption.
-        now eapply prod_ty_inv.
-      + now econstructor.
-      + econstructor.
-        1: now econstructor.
-        eapply typing_subst1.
-        1: now symmetry.
-        econstructor.
-        now eapply prod_ty_inv.
-    - intros * ? []; split; gen_typing.
-    - intros * ? [] ? [] ? [] ? []; split.
-      + now eapply typing_subst1.
-      + gen_typing.
-      + eapply ty_conv.
-        assert [Γ |-[de] tNat ≅ tNat] by now constructor.
-        1: eapply ty_natElim; tea; eapply ty_conv; tea. 
-        * eapply typing_subst1; tea; do 2 constructor; boundary.
-        * eapply elimSuccHypTy_conv ; tea.
-          now boundary.
-        * symmetry; now eapply typing_subst1.
-    - intros **; split; tea.
-      eapply ty_natElim; tea; constructor; boundary.   
-    - intros **.
-      assert [Γ |- tSucc n : tNat] by now constructor.
-      assert [Γ |- P[(tSucc n)..]] by now eapply typing_subst1.
-      split; tea.
-      2: eapply ty_simple_app.
-      1,5: now eapply ty_natElim.
-      2: tea.
-      1: now eapply typing_subst1.
-      replace (arr _ _) with (arr P P[tSucc (tRel 0)]⇑)[n..] by now bsimpl.
-      eapply ty_app; tea.
-    - intros * ? [] ? []; split.
-      + now eapply typing_subst1.
-      + gen_typing.
-      + eapply ty_conv.
-        assert [Γ |-[de] tEmpty ≅ tEmpty] by now constructor.
-        1: eapply ty_emptyElim; tea; eapply ty_conv; tea. 
-        * symmetry; now eapply typing_subst1.
-    - intros * ? [] ? [].
-      split ; gen_typing.
-    - intros * ? [].
-      split ; gen_typing.
-    - intros * ? [] ? [].
-      split ; gen_typing.
+    red; prod_splitter; try now constructor.
+    - intros Γ A t H; apply Fundamental in H as [? VA _].
+      now eapply escapeTy.
+    - intros Γ A B H; apply Fundamental in H as [? VA VB _]; split.
+      + now eapply escapeTy.
+      + now eapply escapeTy.
+    - intros Γ A t u H; apply Fundamental in H as [? VA Vt Vu]; prod_splitter.
+      + now eapply escapeTy.
+      + now eapply escapeTm.
+      + now eapply escapeTm.
   Qed.
 
 End Boundary.
 
-Corollary boundary_tm Γ A t : [Γ |- t : A] -> [Γ |- A].
+Corollary boundary_tm wl Γ A t : [Γ |- t : A]< wl > -> [Γ |- A]< wl >.
 Proof.
   now intros ?%boundary.
 Qed.
 
-Corollary boundary_ty_conv_l Γ A B : [Γ |- A ≅ B] -> [Γ |- A].
+Corollary boundary_ty_conv_l wl Γ A B : [Γ |- A ≅ B]< wl > -> [Γ |- A]< wl >.
 Proof.
   now intros ?%boundary.
 Qed.
 
-Corollary boundary_ty_conv_r Γ A B : [Γ |- A ≅ B] -> [Γ |- B].
+Corollary boundary_ty_conv_r wl Γ A B : [Γ |- A ≅ B]< wl > -> [Γ |- B]< wl >.
 Proof.
   now intros ?%boundary.
 Qed.
 
-Corollary boundary_red_ty_r Γ A B : [Γ |- A ⇒* B] -> [Γ |- B].
+Corollary boundary_red_ty_r wl Γ A B : [Γ |- A ⤳* B]< wl > -> [Γ |- B]< wl >.
 Proof.
   now intros ?%RedConvTyC%boundary.
 Qed.
 
-Corollary boundary_tm_conv_l Γ A t u : [Γ |- t ≅ u : A] -> [Γ |- t : A].
+Corollary boundary_tm_conv_l wl Γ A t u : [Γ |- t ≅ u : A]< wl > -> [Γ |- t : A]< wl >.
 Proof.
   now intros []%boundary.
 Qed.
 
-Corollary boundary_tm_conv_r Γ A t u : [Γ |- t ≅ u : A] -> [Γ |- u : A].
+Corollary boundary_tm_conv_r wl Γ A t u : [Γ |- t ≅ u : A]< wl > -> [Γ |- u : A]< wl >.
 Proof.
   now intros []%boundary.
 Qed.
 
-Corollary boundary_tm_conv_ty Γ A t u : [Γ |- t ≅ u : A] -> [Γ |- A].
+Corollary boundary_tm_conv_ty wl Γ A t u : [Γ |- t ≅ u : A]< wl > -> [Γ |- A]< wl >.
 Proof.
   now intros []%boundary.
 Qed.
 
-Corollary boundary_red_tm_r Γ A t u : [Γ |- t ⇒* u : A] -> [Γ |- u : A].
+Corollary boundary_red_tm_r wl Γ A t u : [Γ |- t ⤳* u : A]< wl > -> [Γ |- u : A]< wl >.
 Proof.
   now intros []%RedConvTeC%boundary.
 Qed.
 
-Corollary boundary_red_tm_ty Γ A t u : [Γ |- t ⇒* u : A] -> [Γ |- A].
+Corollary boundary_red_tm_ty wl Γ A t u : [Γ |- t ⤳* u : A]< wl > -> [Γ |- A]< wl >.
 Proof.
   now intros []%RedConvTeC%boundary.
 Qed.
@@ -440,9 +526,9 @@ Qed.
   boundary_red_tm_l boundary_red_tm_r boundary_red_tm_ty
   boundary_red_ty_r : boundary.
 
-Lemma boundary_ctx_conv_l (Γ Δ : context) :
-  [ |- Γ ≅ Δ] ->
-  [|- Γ].
+Lemma boundary_ctx_conv_l wl (Γ Δ : context) :
+  [ |- Γ ≅ Δ]< wl > ->
+  [|- Γ]< wl >.
 Proof.
   destruct 1.
   all: econstructor ; boundary.
@@ -450,29 +536,17 @@ Qed.
 
 #[export] Hint Resolve boundary_ctx_conv_l : boundary.
 
-Corollary conv_ctx_refl_l (Γ Δ : context) :
-[ |- Γ ≅ Δ] ->
-[|- Γ ≅ Γ].
+Corollary conv_ctx_refl_l wl (Γ Δ : context) :
+[ |- Γ ≅ Δ]< wl > ->
+[|- Γ ≅ Γ]< wl >.
 Proof.
   intros.
   eapply ctx_refl ; boundary.
 Qed.
-
-Lemma typing_eta' (Γ : context) A B f :
-  [Γ |- f : tProd A B] ->
-  [Γ,, A |- eta_expand f : B].
-Proof.
-  intros Hf.
-  eapply typing_eta ; tea.
-  - eapply prod_ty_inv.
-    boundary.
-  - eapply prod_ty_inv.
-    boundary.
-Qed.
-
-Corollary red_ty_compl_prod_r Γ A B T :
-  [Γ |- T ≅ tProd A B] ->
-  ∑ A' B', [× [Γ |- T ⇒* tProd A' B'], [Γ |- A ≅ A'] & [Γ,, A |- B' ≅ B]].
+(*
+Corollary red_ty_compl_prod_r wl Γ A B T :
+  [Γ |- T ≅ tProd A B]< wl > ->
+  ∑ A' B', [× [Γ |- T ⤳* tProd A' B']< wl >, [Γ |- A ≅ A']< wl > & [Γ,, A |- B' ≅ B]]< wl >.
 Proof.
   intros HT.
   symmetry in HT.
@@ -484,53 +558,33 @@ Proof.
   1-2: now boundary.
   now symmetry.
 Qed.
-
+*)
 Section Stability.
 
-  Lemma conv_well_subst (Γ Δ : context) :
-    [ |- Γ ≅ Δ] ->
-    [Γ |-s tRel : Δ].
+  Lemma conv_well_subst (wl : wfLCon) (Γ Δ : context) :
+    [ |- Γ ≅ Δ]< wl > ->
+    [Γ |-s tRel : Δ]< wl >.
   Proof.
-    induction 1 as [| * ? HA].
-    - now econstructor.
-    - assert [Γ |- A] by boundary.
-      assert [|- Γ,, A] by
-        (econstructor ; boundary).
-      econstructor ; tea.
-      + eapply well_subst_ext, well_subst_up ; tea.
-        reflexivity.
-      + eapply wfTermConv.
-        1: econstructor; [gen_typing| now econstructor].
-        rewrite <- rinstInst'_term; do 2 erewrite <- wk1_ren_on.
-        now eapply typing_wk.
+    intros; eapply conv_well_subst; tea; boundary.
   Qed.
 
-  Let PCon (Γ : context) := True.
-  Let PTy (Γ : context) (A : term) := forall Δ,
-    [|- Δ ≅ Γ] -> [Δ |- A].
-  Let PTm (Γ : context) (A t : term) := forall Δ,
-    [|- Δ ≅ Γ] -> [Δ |- t : A].
-  Let PTyEq (Γ : context) (A B : term) := forall Δ,
-    [|- Δ ≅ Γ] -> [Δ |- A ≅ B].
-  Let PTmEq (Γ : context) (A t u : term) := forall Δ,
-    [|- Δ ≅ Γ] -> [Δ |- t ≅ u : A].
+  Let PCon (wl : wfLCon) (Γ : context) := True.
+  Let PTy (wl : wfLCon) (Γ : context) (A : term) := forall Δ,
+    [|- Δ ≅ Γ]< wl > -> [Δ |- A]< wl >.
+  Let PTm (wl : wfLCon) (Γ : context) (A t : term) := forall Δ,
+    [|- Δ ≅ Γ]< wl > -> [Δ |- t : A]< wl >.
+  Let PTyEq (wl : wfLCon) (Γ : context) (A B : term) := forall Δ,
+    [|- Δ ≅ Γ]< wl > -> [Δ |- A ≅ B]< wl >.
+  Let PTmEq (wl : wfLCon) (Γ : context) (A t u : term) := forall Δ,
+    [|- Δ ≅ Γ]< wl > -> [Δ |- t ≅ u : A]< wl >.
 
-  Theorem stability : WfDeclInductionConcl PCon PTy PTm PTyEq PTmEq.
+  Theorem stability wl : WfDeclInductionConcl PCon PTy PTm PTyEq PTmEq wl.
   Proof.
-    red.
-    repeat match goal with |- _ × _ => split end.
-    1: now unfold PCon.
-    all: intros * Hty Δ HΔ.
-    all: pose proof (boundary_ctx_conv_l _ _ HΔ).
-    all: eapply conv_well_subst in HΔ.
-    all: pose proof (subst_refl _ _ _ HΔ).
-    all: eapply typing_subst in Hty ; tea.
-    all: asimpl ; repeat (rewrite idSubst_term in Hty ; [..|reflexivity]).
-    all: try eassumption.
+    red; prod_splitter; intros; red;intros; eapply stability0; tea; boundary.
   Qed.
 
 
-  #[global] Instance ConvCtxSym : Symmetric ConvCtx.
+  #[global] Instance ConvCtxSym (wl : wfLCon) : Symmetric (ConvCtx wl).
   Proof.
     intros Γ Δ.
     induction 1.
@@ -539,16 +593,16 @@ Section Stability.
     now symmetry.
   Qed.
 
-  Corollary conv_ctx_refl_r (Γ Δ : context) :
-    [ |- Γ ≅ Δ] ->
-    [|- Δ ≅ Δ].
+  Corollary conv_ctx_refl_r (wl : wfLCon) (Γ Δ : context) :
+    [ |- Γ ≅ Δ]< wl > ->
+    [|- Δ ≅ Δ]< wl >.
   Proof.
     intros H.
     symmetry in H.
     now eapply ctx_refl ; boundary.
   Qed.
 
-  #[global] Instance ConvCtxTrans : Transitive ConvCtx.
+  #[global] Instance ConvCtxTrans (wl : wfLCon) : Transitive (ConvCtx wl).
   Proof.
     intros Γ1 Γ2 Γ3 H1 H2.
     induction H1 in Γ3, H2 |- *.
@@ -561,23 +615,205 @@ Section Stability.
 
 End Stability.
 
-Lemma termGen' Γ t A :
-[Γ |- t : A] ->
-∑ A', (termGenData Γ t A') × [Γ |- A' ≅ A].
+(** ** Generation *)
+
+(** The generation lemma (the name comes from the PTS literature), gives a 
+stronger inversion principle on typing derivations, that give direct access
+to the last non-conversion rule, and bundle together all conversions.
+
+Note that because we do not yet know that [Γ |- t : T] implies [Γ |- T],
+we cannot use reflexivity in the case where the last rule was not a conversion
+one, and we get the slightly clumsy disjunction of either an equality or a
+conversion proof. We get a better version of generation later on, once we have
+this implication. *)
+
+Inductive termGenData (wl : wfLCon) (Γ : context) : term -> term -> Type :=
+    | termGentRel n decl : [|- Γ]< wl > -> in_ctx Γ n decl -> termGenData wl Γ (tRel n) decl
+    | termGentProd A B : [Γ |- A : U]< wl > -> [Γ,, A |- B : U]< wl > -> termGenData wl Γ (tProd A B) U
+    | termGentLambda A t B : [Γ |- A]< wl > -> [Γ,, A |- t : B]< wl > -> termGenData wl Γ (tLambda A t) (tProd A B)
+    | termGentApp f a A B : [Γ |- f : tProd A B]< wl > -> [Γ |- a : A]< wl > -> termGenData wl Γ (tApp f a) B[a..]
+(*    | termGentSort k A : False -> termGenData wl Γ (tSort k) A*) 
+    | termGentNat : termGenData wl Γ tNat U
+    | termGentZero : termGenData wl Γ tZero tNat
+    | termGentSucc n : [Γ |- n : tNat]< wl > -> termGenData wl Γ (tSucc n) tNat
+    | termGentNatElim P hz hs n :
+      [Γ,, tNat |- P]< wl > -> [Γ |- hz : P[tZero..]]< wl > -> [Γ |- hs : elimSuccHypTy P]< wl > ->
+      [Γ |- n : tNat]< wl > -> termGenData wl Γ (tNatElim P hz hs n) P[n..]
+    | termGentBool : termGenData wl Γ tBool U
+    | termGentTrue : termGenData wl Γ tTrue tBool
+    | termGentFalse : termGenData wl Γ tFalse tBool
+    | termGentBoolElim P ht hf n :
+      [Γ,, tBool |- P]< wl > -> [Γ |- ht : P[tTrue..]]< wl > -> [Γ |- hf : P[tFalse..]]< wl > ->
+      [Γ |- n : tBool]< wl > -> termGenData wl Γ (tBoolElim P ht hf n) P[n..]
+    | termGentAlpha n : [Γ |- n : tNat]< wl > -> termGenData wl Γ (tAlpha n) tBool
+    | termGentEmpty : termGenData wl Γ tEmpty U
+    | termGentEmptyElim P e :
+      [Γ,, tEmpty |- P]< wl > -> [Γ |- e : tEmpty]< wl > -> termGenData wl Γ (tEmptyElim P e) P[e..]
+    | termGentSig A B : [Γ |- A : U]< wl > -> [Γ ,, A |- B : U]< wl > -> termGenData wl Γ (tSig A B) U
+    | termGentPair A B a b :
+      [Γ |- A]< wl > -> [Γ,, A |- B]< wl > -> [Γ |- a : A]< wl > ->
+      [Γ |- b : B[a..]]< wl > -> termGenData wl Γ (tPair A B a b) (tSig A B)
+    | termGentFst p A B : [Γ |- p : tSig A B]< wl > -> termGenData wl Γ (tFst p) A
+    | termGentSnd p A B : [Γ |- p : tSig A B]< wl > -> termGenData wl Γ (tSnd p) B[(tFst p)..]
+    | termGentId A x y : [Γ |- A : U]< wl > -> [Γ |- x : A]< wl > -> [Γ |- y : A]< wl > -> termGenData wl Γ (tId A x y) U
+    | termGentRefl A x : [Γ |- A]< wl > -> [Γ |- x : A]< wl > -> termGenData wl Γ (tRefl A x) (tId A x x)
+    | termGentIdElim A x P hr y e : 
+      [Γ |- A]< wl > -> [Γ |- x : A]< wl > -> [Γ,, A,, tId A⟨@wk1 Γ A⟩ x⟨@wk1 Γ A⟩ (tRel 0) |- P]< wl > ->
+      [Γ |- hr : P[tRefl A x .: x..]]< wl > -> [Γ |- y : A]< wl > -> [Γ |- e : tId A x y]< wl > ->
+      termGenData wl Γ (tIdElim A x P hr y e) P[e .: y..]
+    | ϝtermGen {t A At Af} {n} {ne : not_in_LCon (pi1 wl) n} :
+      [Γ |- At ≅ A]< wl ,,l (ne, true) > ->
+      termGenData (wl ,,l (ne, true)) Γ t At ->
+      [Γ |- Af ≅ A]< wl ,,l (ne, false) > ->
+      termGenData (wl ,,l (ne, false)) Γ t Af ->
+      termGenData wl Γ t A.
+ 
+
+
+
+(*
+Definition termGenData (wl : wfLCon) (Γ : context) (t T : term) : Type :=
+  match t with
+    | tRel n => ∑ decl, [× T = decl, [|- Γ]< wl >& in_ctx Γ n decl]
+    | tProd A B =>  [× T = U, [Γ |- A : U]< wl > & [Γ,, A |- B : U]< wl >]
+    | tLambda A t => ∑ B, [× T = tProd A B, [Γ |- A]< wl > & [Γ,, A |- t : B]< wl >]
+    | tApp f a => ∑ A B, [× T = B[a..], [Γ |- f : tProd A B]< wl > & [Γ |- a : A]< wl >]
+    | tSort _ => False
+    | tNat => T = U
+    | tZero => T = tNat
+    | tSucc n => T = tNat × [Γ |- n : tNat]< wl >
+    | tNatElim P hz hs n =>
+      [× T = P[n..], [Γ,, tNat |- P]< wl >, [Γ |- hz : P[tZero..]]< wl >, [Γ |- hs : elimSuccHypTy P]< wl > & [Γ |- n : tNat]< wl >]
+    | tBool => T = U
+    | tTrue => T = tBool
+    | tFalse => T = tBool
+    | tBoolElim P ht hf n =>
+      [× T = P[n..], [Γ,, tBool |- P]< wl >, [Γ |- ht : P[tTrue..]]< wl >, [Γ |- hf : P[tFalse..]]< wl > & [Γ |- n : tBool]< wl >]
+    | tAlpha n => T = tBool × [Γ |- n : tNat]< wl >
+    | tEmpty => T = U
+    | tEmptyElim P e =>
+      [× T = P[e..], [Γ,, tEmpty |- P]< wl > & [Γ |- e : tEmpty]< wl >]
+    | tSig A B => [× T = U, [Γ |- A : U]< wl > & [Γ ,, A |- B : U]< wl >]
+    | tPair A B a b =>
+     [× T = tSig A B, [Γ |- A]< wl >, [Γ,, A |- B]< wl >, [Γ |- a : A]< wl > & [Γ |- b : B[a..]]< wl >]
+    | tFst p => ∑ A B, T = A × [Γ |- p : tSig A B]< wl >
+    | tSnd p => ∑ A B, T = B[(tFst p)..] × [Γ |- p : tSig A B]< wl >
+    | tId A x y => [× T = U, [Γ |- A : U]< wl >, [Γ |- x : A]< wl > & [Γ |- y : A]< wl >]
+    | tRefl A x => [× T = tId A x x, [Γ |- A]< wl > & [Γ |- x : A]< wl >]
+    | tIdElim A x P hr y e => 
+      [× T = P[e .: y..], [Γ |- A]< wl >, [Γ |- x : A]< wl >, [Γ,, A,, tId A⟨@wk1 Γ A⟩ x⟨@wk1 Γ A⟩ (tRel 0) |- P]< wl >, [Γ |- hr : P[tRefl A x .: x..]]< wl >, [Γ |- y : A]< wl > & [Γ |- e : tId A x y]< wl >]
+  end.
+*)
+
+
+Lemma termGen wl Γ t A :
+  [Γ |- t : A]< wl > ->
+  ∑ A', termGenData wl Γ t A' × ((A' = A) + [Γ |- A' ≅ A]< wl >).
+Proof.
+  induction 1 ; cbn.
+  all: try now (eexists ; split ; [..|left ; reflexivity] ; now econstructor).
+  - destruct IHTypingDecl as [? [? [-> | ]]].
+    + prod_splitter; tea; now right.
+    + prod_splitter; tea; right; now eapply TypeTrans.
+  - eexists ; split ; [..|left ; reflexivity].
+    destruct IHTypingDecl1 as [At [HAt Heqt]] ; destruct IHTypingDecl2 as [Af [HAf Heqf]] ; econstructor.
+    2,4: eassumption.
+    + destruct Heqt ; [ subst | now eauto].
+      econstructor.
+      now boundary.
+    + destruct Heqf ; [ subst | now eauto].
+      econstructor.
+      now boundary.
+Qed.
+
+Lemma neutral_ty_inv wl Γ A :
+  [Γ |- A]< wl > -> whne A -> [Γ |- A : U]< wl >.
+Proof.
+  intros Hty Hne.
+  unshelve eapply TypeRefl, ty_conv_inj in Hty.
+  - now constructor.
+  - now constructor.
+  - cbn in *.
+    apply Fundamental in Hty; destruct Hty.
+    now eapply escapeTm.
+Qed.
+
+Lemma prod_ty_inv wl Γ A B :
+  [Γ |- tProd A B]< wl > ->
+  [Γ |- A]< wl > × [Γ,, A |- B]< wl >.
+Proof.
+  intros Hty.
+  apply Fundamental in Hty; destruct Hty.
+  pose proof (HA := PiValidDom _ VA).
+  pose proof (HB := PiValidCod _ VA).
+  split ; now eapply escapeTy.
+Qed.
+
+Lemma sig_ty_inv wl Γ A B :
+  [Γ |- tSig A B]< wl > ->
+  [Γ |- A]< wl > × [Γ,, A |- B]< wl >.
+Proof.
+  intros Hty.
+  apply Fundamental in Hty; destruct Hty.
+  pose proof (HA := domSigValid _ VA).
+  pose proof (HB := codSigValid _ VA).
+  split ; now eapply escapeTy.
+Qed.
+(*
+Lemma id_ty_inv wl Γ A x y :
+  [Γ |- tId A x y]< wl > ->
+  [Γ |- A]< wl > × [Γ |- x : A]< wl > × [Γ |- y : A]< wl >.
+Proof.
+  intros Hty.
+  apply Fundamental in Hty; destruct Hty.
+  split ; [eapply escapeTy |..].
+  
+  apply TypeRefl id_ty_inj in Hty as [HA HB].
+  prod_splitter; boundary.
+Qed.
+*)
+Lemma termGen' wl Γ t A :
+[Γ |- t : A]< wl > ->
+∑ A', (termGenData wl Γ t A') × [Γ |- A' ≅ A]< wl >.
 Proof.
 intros * H.
-destruct (termGen _ _ _ H) as [? [? [->|]]].
+destruct (termGen _ _ _ _ H) as [? [? [->|]]].
 2: now eexists.
 eexists ; split ; tea.
 econstructor.
 boundary.
 Qed.
 
-Theorem subject_reduction_one Γ A t t' :
-    [Γ |- t : A] ->
-    [t ⇒ t'] ->
-    [Γ |- t ≅ t' : A].
+Lemma typing_eta' (wl : wfLCon) (Γ : context) A B f :
+  [Γ |- f : tProd A B]< wl > ->
+  [Γ,, A |- eta_expand f : B]< wl >.
 Proof.
+  intros Hf.
+  eapply typing_eta ; tea.
+  - eapply prod_ty_inv.
+    boundary.
+  - eapply prod_ty_inv.
+    boundary.
+Qed.
+
+Theorem subject_reduction_one wl Γ A t t' :
+    [Γ |- t : A]< wl > ->
+    [t ⤳ t']< wl > ->
+    [Γ |- t ≅ t' : A]< wl >.
+Proof.
+  intros Hty Hred.
+  destruct (termGen' _ _ _ _ Hty) as [A' [tG Hconv]].
+  induction tG in Hred, Hconv, A |- *.
+  all: try (now inversion Hred).
+  - inversion Hred.
+    + subst.      
+      econstructor ; [ | eassumption].
+      pose proof (boundary_tm _ _ _ _ t).
+      eapply prod_ty_inv in H.
+      econstructor ; eauto.
+      1: 
+      Check eta_expand.
+  
   intros Hty Hred.
   induction Hred in Hty, A |- *.
   - apply termGen' in Hty as (?&((?&?&[-> Hty])&Heq)).
@@ -607,13 +843,46 @@ Proof.
     econstructor.
     1: now econstructor.
     now eapply IHHred.
+  - apply termGen' in Hty as [? [[?[?[->]]]]].
+    eapply TermConv; tea ; refold.
+    now econstructor.
+  - apply termGen' in Hty as [?[[?[?[-> h]]]]].
+    apply termGen' in h as [?[[->] u]].
+    destruct (sig_ty_inj _ _ _ _ _ u).
+    eapply TermConv; refold.
+    2: etransitivity;[|tea]; now symmetry.
+    econstructor; tea.
+  - apply termGen' in Hty as [? [[?[?[->]]]]].
+    eapply TermConv; tea ; refold.
+    now econstructor.
+  - apply termGen' in Hty as [?[[?[?[-> h]]]]].
+    apply termGen' in h as [?[[->] u]].
+    destruct (sig_ty_inj _ _ _ _ _ u).
+    assert [Γ |- B[(tFst (tPair A0 B a b))..] ≅ A]< wl >.
+    1:{ etransitivity; tea. eapply typing_subst1; tea.
+      eapply TermConv; refold. 2: now symmetry.
+      eapply TermRefl; refold; gen_typing.
+    }
+    eapply TermConv; tea; refold.
+    now econstructor.
+  - apply termGen' in Hty as [? [[-> ????? h]]].
+    apply termGen' in h as [? [[->] h']].
+    pose proof h' as []%id_ty_inj.
+    econstructor; tea.
+    econstructor; tea.
+    1: now econstructor.
+    + eapply TermConv; refold; [etransitivity; tea|]; now symmetry.
+    + eapply TermConv; refold; now symmetry.
+  - apply termGen' in Hty as [? [[-> ????? h]]].
+    econstructor; tea; econstructor; tea.
+    all: now first [eapply TypeRefl |eapply TermRefl| eauto].
   Qed.
 
 
-  Theorem subject_reduction_one_type Γ A A' :
-  [Γ |- A] ->
-  [A ⇒ A'] ->
-  [Γ |- A ≅ A'].
+  Theorem subject_reduction_one_type wl Γ A A' :
+  [Γ |- A]< wl > ->
+  [A ⤳ A']< wl > ->
+  [Γ |- A ≅ A']< wl >.
 Proof.
   intros Hty Hred.
   destruct Hred.
@@ -624,9 +893,9 @@ Proof.
 Qed.
 
 Theorem subject_reduction Γ t t' A :
-  [Γ |- t : A] ->
-  [t ⇒* t'] ->
-  [Γ |- t ⇒* t' : A].
+  [Γ |- t : A]< wl > ->
+  [t ⤳* t']< wl > ->
+  [Γ |- t ⤳* t' : A]< wl >.
 Proof.
   intros Hty Hr; split ; refold.
   - assumption.
@@ -639,10 +908,10 @@ Proof.
       now boundary.
 Qed.
 
-Theorem subject_reduction_type Γ A A' :
-[Γ |- A] ->
-[A ⇒* A'] ->
-[Γ |- A ⇒* A'].
+Theorem subject_reduction_type wl Γ A A' :
+[Γ |- A]< wl > ->
+[A ⤳* A']< wl > ->
+[Γ |- A ⤳* A']< wl >.
 Proof.
   intros Hty Hr; split; refold.
   - assumption.
@@ -655,7 +924,7 @@ Proof.
       now boundary.
 Qed.
 
-Corollary conv_red_l Γ A A' A'' : [Γ |-[de] A' ≅ A''] -> [A' ⇒* A] -> [Γ |-[de] A ≅ A''].
+Corollary conv_red_l wl Γ A A' A'' : [Γ |-[de] A' ≅ A'']< wl > -> [A' ⤳* A]< wl > -> [Γ |-[de] A ≅ A'']< wl >.
 Proof.
   intros Hconv **.
   etransitivity ; tea.
@@ -663,3 +932,223 @@ Proof.
   eapply RedConvTyC, subject_reduction_type ; tea.
   boundary.
 Qed.
+
+Lemma Uterm_isType wl Γ A :
+  [Γ |-[de] A : U]< wl > ->
+  whnf A ->
+  isType A.
+Proof.
+  intros Hty Hwh.
+  destruct Hwh.
+  all: try solve [now econstructor].
+  all: exfalso.
+  all: eapply termGen' in Hty ; cbn in *.
+  all: prod_hyp_splitter ; try easy.
+  all: subst.
+  all:
+    match goal with
+      H : [_ |-[de] _ ≅ U] |- _ => unshelve eapply ty_conv_inj in H as Hconv
+    end.
+  all: try now econstructor.
+  all: try now cbn in Hconv.
+Qed.
+  
+Lemma type_isType wl Γ A :
+  [Γ |-[de] A]< wl > ->
+  whnf A ->
+  isType A.
+Proof.
+  intros [] ; refold; cycle -1.
+  1: intros; now eapply Uterm_isType.
+  all: econstructor.
+Qed.
+
+Lemma fun_isFun wl Γ A B t:
+  [Γ |-[de] t : tProd A B]< wl > ->
+  whnf t ->
+  isFun t.
+Proof.
+  intros Hty Hwh.
+  destruct Hwh.
+  all: try now econstructor.
+  all: eapply termGen' in Hty ; cbn in *.
+  all: exfalso.
+  all: prod_hyp_splitter ; try easy.
+  all: subst.
+  all:
+    match goal with
+      H : [_ |-[de] _ ≅ tProd _ _]< wl > |- _ => unshelve eapply ty_conv_inj in H as Hconv
+    end.
+  all: try now econstructor.
+  all: now cbn in Hconv.
+Qed.
+
+Lemma nat_isNat Γ t:
+  [Γ |-[de] t : tNat]< wl > ->
+  whnf t ->
+  isNat t.
+Proof.
+  intros Hty Hwh.
+  destruct Hwh.
+  all: try now econstructor.
+  all: eapply termGen' in Hty ; cbn in *.
+  all: exfalso.
+  all: prod_hyp_splitter ; try easy.
+  all: subst.
+  all:
+    match goal with
+      H : [_ |-[de] _ ≅ tNat]< wl > |- _ => unshelve eapply ty_conv_inj in H as Hconv
+    end.
+  all: try now econstructor.
+  all: now cbn in Hconv.
+Qed.
+
+Lemma empty_isEmpty Γ t:
+  [Γ |-[de] t : tEmpty]< wl > ->
+  whnf t ->
+  whne t.
+Proof.
+  intros Hty Hwh.
+  destruct Hwh ; try easy.
+  all: eapply termGen' in Hty ; cbn in *.
+  all: exfalso.
+  all: prod_hyp_splitter ; try easy.
+  all: subst.
+  all:
+    match goal with
+      H : [_ |-[de] _ ≅ tEmpty]< wl > |- _ => unshelve eapply ty_conv_inj in H as Hconv
+    end.
+  all: try now econstructor.
+  all: now cbn in Hconv.
+Qed.
+
+Lemma id_isId Γ t {A x y} :
+  [Γ |-[de] t : tId A x y]< wl > ->
+  whnf t ->
+  whne t + ∑ A' x', t = tRefl A' x'.
+Proof.
+  intros Hty wh; destruct wh; try easy.
+  all: eapply termGen' in Hty; cbn in *; exfalso.
+  all: prod_hyp_splitter ; try easy; subst.
+  all:
+    match goal with
+      H : [_ |-[de] _ ≅ tId _ _ _]< wl > |- _ => unshelve eapply ty_conv_inj in H as Hconv
+    end; try econstructor.
+  all: now cbn in Hconv.
+Qed.
+
+
+Lemma neutral_isNeutral wl Γ A t :
+  [Γ |-[de] t : A]< wl > ->
+  whne A ->
+  whnf t ->
+  whne t.
+Proof.
+  intros (?&Hgen&Hconv)%termGen' HwA Hwh.
+  set (iA := NeType HwA).
+  destruct Hwh ; cbn in * ; try easy.
+  all: exfalso.
+  all: prod_hyp_splitter.
+  all: subst.
+  all: unshelve eapply ty_conv_inj in Hconv ; tea.
+  all: try now econstructor.
+  all: now cbn in Hconv.
+Qed.
+  Lemma isType_WRed_to_Red : forall (wl : wfLCon) (Γ : context) (T : term) l,
+        isType T ->
+        W[ Γ ||-< l > T ]< wl > ->
+        [ Γ ||-< l > T ]< wl >.
+  Proof.
+    intros ???? [] ; intros Hyp.
+    - destruct s.
+      assert (forall d : DTree wl,
+                 Ssig (fun wl' : wfLCon => over_tree wl wl' d)).
+      { clear.
+        induction d.
+        - exists k.
+          now eapply wfLCon_le_id.
+        - cbn.
+          clear IHd2 ; destruct IHd1 as [wl' Hyp].
+          exists wl'.
+          pose (H := over_tree_le Hyp _ _ (in_here_l _)).
+          now rewrite (decidInLCon_true H).
+      }
+      specialize (H (WT _ Hyp)) as [wl' Ho].
+      pose proof (Red := WRed _ Hyp _ Ho).
+      eapply invLRU in Red ; destruct Red.
+      eapply LRU_.
+      econstructor.
+      1: eassumption.
+      now Wescape ; gen_typing.
+      eapply redtywf_refl ; now Wescape.
+    - assert (WHA : W[ Γ ||-< l > A ]< wl >).
+      { exists (WT _ Hyp).
+        intros wl' Ho ; destruct Hyp as [d Hd] ; cbn in * ; specialize (Hd wl' Ho).
+        eapply invLRΠ in Hd.
+        destruct Hd as [X Y red ????]. Print whnf.
+        pose proof (Heq := redtywf_whnf red (whnf_tProd)) ; inversion Heq ; subst ; clear Heq.
+        destruct polyRed.
+        erewrite <- (wk_id_ren_on Γ X).
+        eapply shpRed.
+        1: now eapply wfLCon_le_id.
+        gen_typing.
+      }
+      assert (WHB : W[ Γ,, A ||-< l > B ]< wl >) by admit.
+      eapply LRPi'.
+      econstructor ; [ .. | unshelve econstructor].
+      1: eapply redtywf_refl ; now Wescape.
+      1,2: econstructor ; now Wescape.
+      5,6: now Wescape.
+      + econstructor ; now Wescape.
+      + 
+      
+      { eapply (TreeSplit (WT _ Hyp)).
+        intros wl' Ho ; destruct Hyp as [d Hd] ; cbn in * ; specialize (Hd wl' Ho).
+        eapply invLRΠ in Hd.
+        destruct Hd as [X Y red ????]. Print whnf.
+        pose proof (Heq := redtywf_whnf red (whnf_tProd)) ; inversion Heq ; subst ; clear Heq.
+        destruct polyRed.
+        About FundTmVar.
+        Print FundTm.
+        About PiValidCod.
+        erewrite <- (wk_id_ren_on Γ X).
+        eapply shpRed.
+        1: now eapply wfLCon_le_id.
+        
+        
+        Print wk_id.
+        Unset Printing Notations. Print wk_well_wk.
+
+      Wescape.
+      eapply LRPi'.
+      cbn.
+      econstructor.
+      1: now eapply redtywf_refl.
+      gen_typing.
+      1: as.
+
+      About LRLRΠ_.
+
+      ∑ wl', [ Γ ||-< l > U ]< wl' >).
+      { destruct Hyp as [d Hd].
+        unshelve eexists _ ; [ | eapply Hd].
+        Print DTree.
+        all: clear Hd.
+        revert wl d.
+        refine (fix f wl d := match d as d0 in (DTree _) return wfLCon with
+                              | leaf _ => _
+                              | @ϝnode _ n ne dt df => _
+                              end).
+                             ; induction d.
+        + assumption.
+        + unshelve eapply wfLCons ; [exact IHd1 | .. ].
+          exact IHd1.
+        + now eapply wfLCon_le_id.
+        + cbn.
+        
+      About WUnivEq.
+      pose (wl' := DTree_path _ _ (WT _ Hyp)).
+      About DTree_path.
+      Print invLRU.
+      eapply LRU_.
+      econstructor.
